code/sha3/Hacl.Hash.SHA3.Simd256.fst
@@ -18,8 +18,10 @@ open Hacl.Spec.SHA3.Vec.Common
 open Hacl.Impl.SHA3.Vec
 
 module S = Spec.SHA3
+module V = Hacl.Spec.SHA3.Vec
 module ST = FStar.HyperStack.ST
 module B = LowStar.Buffer
+module M = LowStar.Modifies
 
 #reset-options "--z3rlimit 50 --max_fuel 0 --max_ifuel 0 --using_facts_from '* -FStar.Seq'"
 
@@ -254,3 +256,98 @@ let sha3_512 output0 output1 output2 output3
   let ib = ntup4 (input0,(input1,(input2,input3))) in
   let rb = ntup4 (output0,(output1,(output2,output3))) in
   keccak #SHA3_512 #M256 576ul (* 1024ul *) inputByteLen ib (byte 0x06) 64ul rb
+
+val state_malloc:
+    r:rid
+  -> ST.ST (s:buffer uint64 { length s = 100 })
+  (requires (fun _ ->
+    ST.is_eternal_region r))
+  (ensures (fun h0 s h1 ->
+    live h1 s /\
+    M.(modifies loc_none h0 h1) /\
+    fresh_loc (loc_addr_of_buffer s) h0 h1 /\
+    (M.loc_includes (M.loc_region_only true r) (loc_addr_of_buffer s)) /\
+    freeable s))
+
+let state_malloc r =
+  malloc r (u64 0) 100ul
+
+val state_free:
+    s:buffer uint64 { length s = 100 }
+  -> ST.ST unit
+  (requires fun h0 ->
+    freeable s /\ live h0 s)
+  (ensures fun h0 _ h1 ->
+    M.modifies (loc_addr_of_buffer s) h0 h1)
+
+let state_free s =
+  free s
+
+open Lib.NTuple
+open Lib.MultiBuffer
+open Lib.IntVector
+
+val shake128_absorb:
+  state:lbuffer_t MUT (vec_t U64 4) 25ul
+  -> input0:buffer_t MUT uint8
+  -> input1:buffer_t MUT uint8
+  -> input2:buffer_t MUT uint8
+  -> input3:buffer_t MUT uint8
+  -> inputByteLen:size_t{v inputByteLen == length input0 /\ 
+                         v inputByteLen == length input1 /\
+                         v inputByteLen == length input2 /\
+                         v inputByteLen == length input3}
+  -> Stack unit
+     (requires fun h ->
+       live4 h (input0 <: lbuffer uint8 inputByteLen)
+               (input1 <: lbuffer uint8 inputByteLen)
+               (input2 <: lbuffer uint8 inputByteLen)
+               (input3 <: lbuffer uint8 inputByteLen) /\
+       live h state /\
+       disjoint input0 state /\
+       disjoint input1 state /\
+       disjoint input2 state /\
+       disjoint input3 state)
+     (ensures  fun h0 _ h1 ->
+       modifies (loc state) h0 h1 /\
+       as_seq h1 state ==
+          V.absorb #Shake128 #M256 (as_seq h0 state) 168 (v inputByteLen) (as_seq_multi h0 (ntup4 (input0, (input1, (input2, input3))))) (byte 0x1F))
+let shake128_absorb state input0 input1 input2 input3 inputByteLen =
+  absorb #Shake128 #M256 168ul inputByteLen (ntup4 (input0, (input1, (input2, input3)))) (byte 0x1F) state
+
+val shake128_squeeze_nblocks:
+  state:lbuffer_t MUT (vec_t U64 4) 25ul
+  -> output0:buffer_t MUT uint8
+  -> output1:buffer_t MUT uint8
+  -> output2:buffer_t MUT uint8
+  -> output3:buffer_t MUT uint8
+  -> outputByteLen:size_t{v outputByteLen == length output0 /\ 
+                          v outputByteLen == length output1 /\
+                          v outputByteLen == length output2 /\
+                          v outputByteLen == length output3}
+  -> Stack unit
+     (requires fun h ->
+       live4 h (output0 <: lbuffer uint8 outputByteLen)
+               (output1 <: lbuffer uint8 outputByteLen)
+               (output2 <: lbuffer uint8 outputByteLen)
+               (output3 <: lbuffer uint8 outputByteLen) /\
+       live h state /\
+       disjoint output0 output1 /\
+       disjoint output0 output2 /\
+       disjoint output0 output3 /\
+       disjoint output1 output2 /\
+       disjoint output1 output3 /\
+       disjoint output2 output3 /\
+       disjoint output0 state /\
+       disjoint output1 state /\
+       disjoint output2 state /\
+       disjoint output3 state)
+     (ensures  fun h0 _ h1 ->
+       modifies (loc state |+| loc output0 |+| loc output1 |+| loc output2 |+| loc output3) h0 h1 /\
+       (let s', b' = 
+          V.squeeze_nblocks #Shake128 #M256 168 (v outputByteLen) (as_seq h0 state, as_seq_multi h0 (ntup4 (output0, (output1, (output2, output3))))) in
+          as_seq h1 state == s' /\
+          as_seq_multi h1 (ntup4 (output0, (output1, (output2, output3)))) == b'))
+let shake128_squeeze_nblocks state output0 output1 output2 output3 outputByteLen =
+  loc_multi4 #4 #outputByteLen (ntup4 (output0, (output1, (output2, output3))));
+  squeeze_nblocks #Shake128 #M256 state 168ul outputByteLen (ntup4 (output0, (output1, (output2, output3))))
